src/program_proof/atomic_commit.v
@@ -2,3 +2,134 @@ From Perennial.program_proof Require Import grove_prelude.
 From iris.base_logic Require Export lib.ghost_var.
 From Perennial.program_proof.grove_shared Require Import urpc_proof urpc_spec.
 From Goose.github_com.mit_pdos.gokv Require Import tutorial.
+
+Module decision.
+  Inductive t := Unknown | Commit | Abrt.
+  Definition is_byte (x:t) (b: u8) :=
+    match x with
+    | Unknown => b = U8 0
+    | Commit => b = U8 1
+    | Abrt => b = U8 2
+    end.
+End decision.
+
+(* PLAN:
+
+- start by giving the participant a spec
+- will have a single piece of ghost state for the global preferences
+
+One gname for each participant
+participant ghost state is a single agree(bool) for its preference
+
+also a global decision ghost variable that reflects all of the preferences
+
+Three parallel lists at the coordinator:
+- physical list of decisions
+- physical list of participant clerks
+- ghost list of participant gnames
+
+coordinator's one-shot decision
+
+ *)
+
+Module global_names.
+  Record t :=
+    mk { decision: gname; }.
+End global_names.
+
+Module participant_names.
+  Record t :=
+    mk { preference: gname;
+         urpc: server_chan_gnames; }.
+End participant_names.
+
+Module coordinator_names.
+  Record t :=
+    mk { participants: list gname;
+         globals: global_names.t;
+        }.
+End coordinator_names.
+
+Section iris.
+  Context `{!heapGS Σ}.
+  Context `{!urpcregG Σ}.
+  Context `{inG Σ (agreeR boolO)}.
+
+  Definition is_preference (γ: participant_names.t) (pref: bool) : iProp Σ :=
+    own γ.(participant_names.preference) (to_agree pref).
+
+  Definition is_decision (γ: coordinator_names.t) (decision: bool) : iProp Σ :=
+    own γ.(coordinator_names.globals).(global_names.decision) (to_agree decision).
+
+  Program Definition GetPreference_spec (γ: participant_names.t)
+    : list u8 → (list u8 -d> iProp Σ) -d> iProp Σ :=
+    λ reqData, λne (Φ: list u8 -d> iPropO Σ),
+      (* ignore request *)
+      (∀ (pref: bool), is_preference γ pref -∗
+      Φ (if pref then [U8 1] else [U8 0]))%I.
+  Next Obligation. solve_proper. Defined.
+
+  Definition is_participant_host (γ: participant_names.t) (host:u64) : iProp Σ :=
+    "#H0" ∷ handler_spec γ.(participant_names.urpc) host (U64 0) (GetPreference_spec γ) ∗
+    "#Hdom" ∷ handlers_dom γ.(participant_names.urpc) {[ (U64 0) ]}.
+
+  Definition is_participant_clerk (ck: loc) (γ: participant_names.t) : iProp Σ :=
+    ∃ (cl:loc) host,
+      "#client" ∷ readonly (ck ↦[ParticipantClerk :: "client"] #cl) ∗
+      "#Hhost" ∷ is_participant_host γ host ∗
+      "#His_cl" ∷ is_uRPCClient cl host.
+
+  Lemma wp_ParticipantClerk_GetPreference ck γ :
+    is_participant_clerk ck γ -∗
+    {{{ True }}}
+      ParticipantClerk__GetPreference #ck
+    {{{ (pref: bool), RET #pref;
+        is_preference γ pref
+    }}}.
+  Proof.
+    iIntros "#Hclerk".
+    iIntros (Φ) "!> _ HΦ".
+
+    wp_apply (wp_frame_wand with "HΦ").
+
+    wp_lam.
+    wp_apply wp_NewSlice. iIntros (req_s) "Hreq".
+    wp_pures.
+    wp_apply wp_NewSlice. iIntros (reply_s) "Hreply".
+    rewrite replicate_0.
+    wp_apply wp_ref_to.
+    { val_ty. }
+    iIntros (reply_l) "Hreply_l".
+    wp_pures.
+    iNamed "Hclerk".
+    wp_loadField.
+
+    wp_apply (wp_Client__Call2 with "[] [] [Hreq] Hreply_l").
+    { iFrame "#". }
+    { iNamed "Hhost".
+      iFrame "#". }
+    { admit. (* get is_slice_small *) }
+
+    - iIntros "!> !>".
+      cbn.
+      iIntros (pref) "#Hpref _".
+  Admitted.
+
+  Definition is_coord_clerk (ck: loc) (γ: coordinator_names.t) : iProp Σ := True.
+
+  Lemma wp_CoordinatorClerk_GetDecision ck γ :
+    is_coord_clerk ck γ -∗
+    {{{ True }}}
+      CoordinatorClerk__GetDecision #ck
+    {{{ (decision: decision.t) (b: u8), RET #b;
+        ⌜decision.is_byte decision b⌝ ∗
+        match decision with
+        | decision.Commit => is_decision γ true
+        | decision.Abrt => is_decision γ false
+        | decision.Unknown => True
+        end
+    }}}.
+  Proof.
+  Admitted.
+
+End iris.
